SepLogicTime/Sep_Time_Automation.thy
@@ -1,0 +1,1087 @@
+theory Sep_Time_Automation
+imports
+  "HOL-Eisbach.Eisbach" Sep_Time_Misc   Automatic_Refinement.Automatic_Refinement
+ 
+begin
+
+
+subsection \<open>Experiment TOMOVE\<close>
+lemma run_and_execute: "(\<forall>\<sigma> t r. run c (Some h) \<sigma> r t \<longrightarrow> \<sigma> \<noteq> None \<and> P (the \<sigma>) r t)
+        \<longleftrightarrow> (\<exists>h' t r. execute c h = Some (r, h', t) \<and> P h' r t)"  
+  apply rule
+  subgoal by (metis option.sel run.intros(2) run.intros(3) timeFrame.elims) 
+  subgoal by (metis (mono_tags) not_None_eq option.sel prod.sel(1) prod.sel(2) run_to_execute) 
+  done
+
+
+subsection \<open>stuff for VCG\<close>
+
+lemma is_hoare_triple: "<P> c <Q> \<Longrightarrow> <P> c <Q>" .
+
+theorem normalize_rules:
+           "\<And>P. (\<And>x. <P x> f <Q>) \<Longrightarrow> <\<exists>\<^sub>Ax. P x> f <Q>"
+           "\<And>P. (b \<Longrightarrow> <P> f <Q>) \<Longrightarrow> <P * \<up> b> f <Q>"
+           "\<And>P. (b \<Longrightarrow> <emp> f <Q>) \<Longrightarrow> <\<up> b> f <Q>"
+  subgoal using pre_ex_rule by force
+  subgoal using norm_pre_pure_iff by blast
+  subgoal using norm_pre_pure_iff2 by blast
+  done
+    
+
+subsection "Rotate method"
+
+definition gr where "gr A B = A * B"
+
+lemma right_swap: "(A \<Longrightarrow>\<^sub>A B * (C * D)) \<Longrightarrow> (A \<Longrightarrow>\<^sub>A B * (D * C))"
+  by (simp add: assn_times_comm)
+lemma right_take: "(A \<Longrightarrow>\<^sub>A gr B C * D) \<Longrightarrow> (A \<Longrightarrow>\<^sub>A B * (C * D))"
+  by (simp add: gr_def assn_times_assoc) 
+lemma left_swap: "(B * (C * D) \<Longrightarrow>\<^sub>A A) \<Longrightarrow> (B * (D * C) \<Longrightarrow>\<^sub>A A)"
+  by (simp add: assn_times_comm)
+lemma left_take: "(gr B C * D \<Longrightarrow>\<^sub>A A) \<Longrightarrow> (B * (C * D) \<Longrightarrow>\<^sub>A A)"
+  by (simp add: gr_def assn_times_assoc) 
+
+lemma right_move_back: "(A \<Longrightarrow>\<^sub>A B * C) \<Longrightarrow> (A \<Longrightarrow>\<^sub>A C * B)"
+  by (simp add: assn_times_comm)
+lemma left_move_back: "(B * C \<Longrightarrow>\<^sub>A A) \<Longrightarrow> (C * B \<Longrightarrow>\<^sub>A A)"
+  by (simp add: assn_times_comm)
+lemma right_move_backt: "(A \<Longrightarrow>\<^sub>t B * C) \<Longrightarrow> (A \<Longrightarrow>\<^sub>t C * B)"
+  by (simp add: assn_times_comm)
+lemma left_move_backt: "(B * C \<Longrightarrow>\<^sub>t A) \<Longrightarrow> (C * B \<Longrightarrow>\<^sub>t A)"
+  by (simp add: assn_times_comm)
+
+thm mult.assoc
+method rotater = ( (simp only: mult.assoc)? , rule right_move_back , (simp only: mult.assoc)?  )
+method rotatel = ( (simp only: mult.assoc)? , rule left_move_back , (simp only: mult.assoc)?  )
+
+method swapl = ( (simp only: mult.assoc)? ,rule left_swap, (simp only: mult.assoc)?   )
+method takel = ( (simp only: mult.assoc)? , rule left_take, (simp only: mult.assoc)?  )
+
+method swapr = ( (simp only: mult.assoc)? , rule right_swap , (simp only: mult.assoc)?  )
+method taker = ( (simp only: mult.assoc)? , rule right_take, (simp only: mult.assoc)?  )
+
+method rotatert = ( (simp only: mult.assoc)? , rule right_move_backt , (simp only: mult.assoc)?  )
+method rotatelt = ( (simp only: mult.assoc)? , rule left_move_backt , (simp only: mult.assoc)?  )
+
+
+lemma match_firstt: "A \<Longrightarrow>\<^sub>t B \<Longrightarrow> \<Gamma> * A \<Longrightarrow>\<^sub>t \<Gamma> * B"   
+  by (simp add: entt_star_mono) 
+
+lemma match_restt: "emp \<Longrightarrow>\<^sub>t B \<Longrightarrow> \<Gamma> \<Longrightarrow>\<^sub>t \<Gamma> * B"  
+  using match_firstt by fastforce 
+
+lemma match_first: "A \<Longrightarrow>\<^sub>A B \<Longrightarrow> \<Gamma> * A \<Longrightarrow>\<^sub>A \<Gamma> * B"  
+  by (simp add: assn_times_comm entails_frame)  
+
+lemma match_rest: "emp \<Longrightarrow>\<^sub>A B \<Longrightarrow> \<Gamma> \<Longrightarrow>\<^sub>A \<Gamma> * B"  
+  using match_first by fastforce 
+
+
+
+
+
+subsection "Simplifier setup"
+
+
+lemma is_entails: "P\<Longrightarrow>\<^sub>AQ \<Longrightarrow> P \<Longrightarrow>\<^sub>AQ" .
+ 
+text \<open>Used by existential quantifier extraction tactic\<close>
+lemma enorm_exI': (* Incomplete, as chosen x may depend on heap! *)
+  "(\<And>x. Z x \<longrightarrow> (P \<Longrightarrow>\<^sub>A Q x)) \<Longrightarrow> (\<exists>x. Z x) \<longrightarrow> (P \<Longrightarrow>\<^sub>A (\<exists>\<^sub>Ax. Q x))"
+  by (metis ent_ex_postI)
+
+
+
+lemmas solve_ent_preprocess_simps = 
+  ent_pure_post_iff ent_pure_post_iff_sng ent_pure_pre_iff ent_pure_pre_iff_sng
+lemmas ent_refl = entails_triv
+lemmas ent_triv = ent_true ent_false
+lemmas norm_assertion_simps =
+  (* Neutral elements *)
+  mult_1[where 'a=assn] mult_1_right[where 'a=assn]
+
+  (* Zero elements *)
+  false_absorb star_false_right
+
+  time_credit_add[symmetric]
+  ex_assn_move_out(1) pure_conj[symmetric]
+
+  (* Duplicated References *)
+  sngr_same_false snga_same_false
+
+(*
+theorem solve_ent_preprocess_simps:
+            (?P \<Longrightarrow>\<^sub>A ?Q * \<up> ?b) = ((\<forall>h. h \<Turnstile> ?P \<longrightarrow> ?b) \<and> (?P \<Longrightarrow>\<^sub>A ?Q))
+            (?P \<Longrightarrow>\<^sub>A \<up> ?b) = ((\<forall>h. h \<Turnstile> ?P \<longrightarrow> ?b) \<and> (?P \<Longrightarrow>\<^sub>A emp))
+            (?P * \<up> ?b \<Longrightarrow>\<^sub>A ?Q) = (?b \<longrightarrow> (?P \<Longrightarrow>\<^sub>A ?Q))
+            (\<up> ?b \<Longrightarrow>\<^sub>A ?Q) = (?b \<longrightarrow> (emp \<Longrightarrow>\<^sub>A ?Q)) *) 
+
+
+subsection \<open>Frame Matcher\<close>
+text \<open>Given star-lists P,Q and a frame F, this method tries to match 
+  all elements of Q with corresponding elements of P. The result is a 
+  partial match, that contains matching pairs and the unmatched content.\<close>
+
+text \<open>The frame-matcher internally uses syntactic lists separated by
+  star, and delimited by the special symbol \<open>SLN\<close>, which is defined
+  to be \<open>emp\<close>.\<close>
+definition [simp]: "SLN \<equiv> emp"
+lemma SLN_left: "SLN * P = P" by simp
+lemma SLN_right: "P * SLN = P" by simp
+
+lemmas SLN_normalize = SLN_right mult.assoc[symmetric, where 'a=assn]
+lemmas SLN_strip = SLN_right SLN_left mult.assoc[symmetric, where 'a=assn]
+
+text \<open>A query to the frame matcher. Contains the assertions
+  P and Q that shall be matched, as well as a frame F, that is not 
+  touched.\<close>
+
+definition [simp]: "FI_QUERY P Q F \<equiv> P \<Longrightarrow>\<^sub>A Q*F"
+
+abbreviation "fi_m_fst M \<equiv> foldr ((*)) (map fst M) emp"
+abbreviation "fi_m_snd M \<equiv> foldr ((*)) (map snd M) emp"
+abbreviation "fi_m_match M \<equiv> (\<forall>(p,q)\<in>set M. p \<Longrightarrow>\<^sub>A q)"
+
+text \<open>A result of the frame matcher. Contains a list of matching pairs,
+  as well as the unmatched parts of P and Q, and the frame F.
+\<close>
+definition [simp]: "FI_RESULT M UP UQ F \<equiv> 
+  fi_m_match M \<longrightarrow> (fi_m_fst M * UP \<Longrightarrow>\<^sub>A fi_m_snd M * UQ * F)"
+
+text \<open>Internal structure used by the frame matcher: 
+  m contains the matched pairs; p,q the assertions that still needs to be 
+  matched; up,uq the assertions that could not be matched; and f the frame.
+  p and q are SLN-delimited syntactic lists. 
+\<close>
+
+definition [simp]: "FI m p q up uq f \<equiv> 
+  fi_m_match m \<longrightarrow> (fi_m_fst m * p * up \<Longrightarrow>\<^sub>A fi_m_snd m * q * uq * f)"
+
+text \<open>Initialize processing of query\<close>
+lemma FI_init: 
+  assumes "FI [] (SLN*P) (SLN*Q) SLN SLN F"
+  shows "FI_QUERY P Q F"
+  using assms by simp
+
+text \<open>Construct result from internal representation\<close>
+lemma FI_finalize:
+  assumes "FI_RESULT m (p*up) (q*uq) f"
+  shows "FI m p q up uq f"
+  using assms by (simp add: mult.assoc )
+
+text \<open>Auxiliary lemma to show that all matching pairs together form
+  an entailment. This is required for most applications.\<close>
+lemma fi_match_entails:
+  assumes "fi_m_match m"
+  shows "fi_m_fst m \<Longrightarrow>\<^sub>A fi_m_snd m"
+  using assms apply (induct m)
+  apply (simp_all split: prod.split_asm add: ent_star_mono)
+  done
+
+text \<open>Internally, the frame matcher tries to match the first assertion
+  of q with the first assertion of p. If no match is found, the first
+  assertion of p is discarded. If no match for any assertion in p can be
+  found, the first assertion of q is discarded.\<close>
+
+text \<open>Match\<close>
+lemma FI_match:
+  assumes "p \<Longrightarrow>\<^sub>A q"
+  assumes "FI ((p,q)#m) (ps*up) (qs*uq) SLN SLN f"
+  shows "FI m (ps*p) (qs*q) up uq f"
+  using assms unfolding FI_def
+  apply (simp add: mult.assoc) 
+  by (simp add: mult.left_commute) 
+
+text \<open>No match\<close>
+lemma FI_p_nomatch:
+  assumes "FI m ps (qs*q) (p*up) uq f"
+  shows "FI m (ps*p) (qs*q) up uq f"
+  using assms unfolding FI_def
+  by (simp add: mult.assoc)  
+
+text \<open>Head of q could not be matched\<close>
+lemma FI_q_nomatch:
+  assumes "FI m (SLN*up) qs SLN (q*uq) f"
+  shows "FI m SLN (qs*q) up uq f"
+  using assms unfolding FI_def
+  by (simp add: mult.assoc)  
+
+subsection \<open>Frame Inference\<close>
+lemma frame_inference_init:
+  assumes "FI_QUERY P Q F"
+  shows "P \<Longrightarrow>\<^sub>A Q * F"
+  using assms by simp
+
+lemma frame_inference_finalize:
+  shows "FI_RESULT M F emp F"
+  apply simp
+  apply rule
+  apply (drule fi_match_entails)
+  apply (rule ent_star_mono[OF _ ent_refl])
+  apply assumption
+  done
+
+
+
+subsection \<open>Frame Inference\<close>
+
+definition [simp]: "TI_QUERY P Q F \<equiv> P = Q + F"
+lemma TI_QUERYD: "P = Q + F \<Longrightarrow> TI_QUERY P Q F" by simp
+
+lemma timeframe_inference_init:
+  assumes
+      "FI_QUERY P Q FH"   (* first do frame inference in order to instatiate schematics! *)
+      "TI_QUERY T T' FT"
+      "F = FH * $FT"
+  shows "P * $T\<Longrightarrow>\<^sub>A (Q * F) * $T'"
+  using assms apply (simp add: time_credit_add mult.assoc)
+  apply(rotater) apply rotater apply rotatel apply rotatel apply(rule match_first)  apply rotatel apply (rule match_first)
+  .
+
+lemma timeframe_inference_init_normalize:
+ "emp * $T\<Longrightarrow>\<^sub>A F * $T' \<Longrightarrow> $T\<Longrightarrow>\<^sub>A F * $T'"
+  by auto
+
+
+lemma dollarD: "a = b \<Longrightarrow> $a \<Longrightarrow>\<^sub>A $b"
+  by simp
+
+subsection \<open>Entailment Solver\<close>
+lemma entails_solve_init:
+  "FI_QUERY P (Q*$T) true \<Longrightarrow> P \<Longrightarrow>\<^sub>A Q * true * $T"
+  "FI_QUERY P Q true \<Longrightarrow> P \<Longrightarrow>\<^sub>A Q * true"
+  "FI_QUERY P Q emp \<Longrightarrow> P \<Longrightarrow>\<^sub>A Q"
+    apply (simp_all add: mult.assoc )   
+  by (simp add:  mult.commute)  
+
+lemma entails_solve_init_time':
+  "FI_QUERY P (Q) true \<Longrightarrow> TI_QUERY T T' FT \<Longrightarrow>  P * $T \<Longrightarrow>\<^sub>A Q * true * $T'"
+  apply simp 
+  by (smt ent_star_mono gc_time le_add1 merge_true_star star_aci(2) star_aci(3))
+
+lemma entails_solve_init_time:
+  "FI_QUERY P (Q) true \<Longrightarrow> TI_QUERY T T' FT \<Longrightarrow>  P * $T \<Longrightarrow>\<^sub>A Q * true * $T'"
+  "FI_QUERY P emp true \<Longrightarrow> TI_QUERY T T' FT \<Longrightarrow>  P * $T \<Longrightarrow>\<^sub>A true * $T'"
+  "FI_QUERY emp Q true \<Longrightarrow> TI_QUERY T T' FT \<Longrightarrow>  $T \<Longrightarrow>\<^sub>A Q * true * $T'"
+  "FI_QUERY emp Q true \<Longrightarrow> TI_QUERY T T' FT \<Longrightarrow>  $T \<Longrightarrow>\<^sub>A true * $T'"
+  subgoal by(fact entails_solve_init_time')
+  subgoal using entails_solve_init_time'[where Q=emp] by simp
+  subgoal using entails_solve_init_time'[where P=emp] by simp
+  subgoal using entails_solve_init_time'[where P=emp and Q=emp] by simp
+  done
+
+lemma entails_solve_finalize:
+  "FI_RESULT M P emp true"
+  "FI_RESULT M emp emp emp"
+  by (auto simp add: fi_match_entails intro: ent_star_mono)
+
+
+named_theorems sep_dflt_simps "Seplogic: Default simplification rules for automated solvers"
+named_theorems sep_eintros "Seplogic: Intro rules for entailment solver"
+named_theorems sep_heap_rules "Seplogic: VCG heap rules"
+named_theorems sep_decon_rules "Seplogic: VCG deconstruct rules"
+
+
+
+
+ML \<open>
+infix 1 THEN_IGNORE_NEWGOALS
+
+structure Seplogic_Auto =
+struct
+
+
+  (***********************************)
+  (*          Method Setup           *)
+  (***********************************)
+
+  val dflt_simps_modifiers = [
+    Args.$$$ "dflt_simps" -- Scan.option Args.add -- Args.colon 
+      >> K (Method.modifier (Named_Theorems.add @{named_theorems sep_dflt_simps}) \<^here>),
+    Args.$$$ "dflt_simps" -- Scan.option Args.del -- Args.colon 
+      >> K (Method.modifier (Named_Theorems.del @{named_theorems sep_dflt_simps}) \<^here>)
+  ];
+  val heap_modifiers = [
+    Args.$$$ "heap" -- Scan.option Args.add -- Args.colon 
+      >> K (Method.modifier (Named_Theorems.add @{named_theorems sep_heap_rules}) \<^here>),
+    Args.$$$ "heap" -- Scan.option Args.del -- Args.colon 
+      >> K (Method.modifier (Named_Theorems.del @{named_theorems sep_heap_rules}) \<^here>)
+  ];
+  val decon_modifiers = [
+    Args.$$$ "decon" -- Scan.option Args.add -- Args.colon 
+      >> K (Method.modifier (Named_Theorems.add @{named_theorems sep_decon_rules}) \<^here>),
+    Args.$$$ "decon" -- Scan.option Args.del -- Args.colon 
+      >> K (Method.modifier (Named_Theorems.del @{named_theorems sep_decon_rules}) \<^here>)
+  ];
+
+  val eintros_modifiers = [
+    Args.$$$ "eintros" -- Scan.option Args.add -- Args.colon 
+      >> K (Method.modifier (Named_Theorems.add @{named_theorems sep_eintros}) \<^here>),
+    Args.$$$ "eintros" -- Scan.option Args.del -- Args.colon 
+      >> K (Method.modifier (Named_Theorems.del @{named_theorems sep_eintros}) \<^here>)
+  ];
+
+  val solve_entails_modifiers = dflt_simps_modifiers @ eintros_modifiers;
+
+  val vcg_modifiers = 
+    heap_modifiers @ decon_modifiers @ dflt_simps_modifiers;
+
+  val sep_auto_modifiers = 
+    clasimp_modifiers @ vcg_modifiers @ eintros_modifiers;
+
+
+  (***********************************)
+  (*        Custom Tacticals         *)
+  (***********************************)
+
+  (* Apply tac1, and then tac2 with an offset such that anything left 
+     over by tac1 is skipped.
+
+     The typical usage of this tactic is, if a theorem is instantiated
+     with another theorem that produces additional goals that should 
+     be ignored first. Here, it is used in the vcg to ensure that 
+     frame inference is done before additional premises (that may 
+     depend on the frame) are discharged.
+  *)
+  fun (tac1 THEN_IGNORE_NEWGOALS tac2) i st = let
+    val np = Thm.nprems_of st
+  in
+    (tac1 i THEN (fn st' => let val np' = Thm.nprems_of st' in
+      if np'<np then tac2 i st'
+      else tac2 (i+(np'-np)+1) st'
+    end)) st
+  end;
+
+  (***********************************)
+  (*     Assertion Normalization     *)
+  (***********************************)
+  (* Find two terms in a list whose key is equal *)
+  fun find_similar (key_of:term -> term) (ts:term list) = let
+    fun frec _ [] = NONE
+    | frec tab (t::ts) = let val k=key_of t in
+      if Termtab.defined tab k then
+        SOME (the (Termtab.lookup tab k),t)
+      else frec (Termtab.update (k,t) tab) ts
+    end
+  in
+    frec Termtab.empty ts
+  end;
+
+  (* Perform DFS over term with binary operator opN, threading through
+    a state. Atomic terms are transformed by tr. Supports omission of
+    terms from the result structure by transforming them to NONE. *)
+  fun dfs_opr opN (tr:'state -> term -> ('state*term option)) 
+    d (t as ((op_t as Const (fN,_))$t1$t2)) =
+    if fN = opN then let
+        val (d1,t1') = dfs_opr opN tr d t1;
+        val (d2,t2') = dfs_opr opN tr d1 t2;
+      in
+        case (t1',t2') of
+          (NONE,NONE) => (d2,NONE)
+        | (SOME t1',NONE) => (d2,SOME t1')
+        | (NONE,SOME t2') => (d2,SOME t2')
+        | (SOME t1',SOME t2') => (d2,SOME (op_t$t1'$t2'))
+      end
+    else tr d t
+  | dfs_opr _ tr d t = tr d t;
+    
+  (* Replace single occurrence of (atomic) ot in t by nt. 
+    Returns new term or NONE if nothing was removed. *)
+  fun dfs_replace_atomic opN ot nt t = let
+    fun tr d t = if not d andalso t=ot then (true,SOME nt) else (d,SOME t);
+    val (success,SOME t') = dfs_opr opN tr false t; 
+  in
+    if success then SOME t' else NONE
+  end;
+
+  fun assn_simproc_fun ctxt credex = let
+    val ([redex],ctxt') = Variable.import_terms true [Thm.term_of credex] ctxt;
+    val export = singleton (Variable.export ctxt' ctxt)
+
+    fun mk_star t1 t2 = @{term "(*)::assn \<Rightarrow> _ \<Rightarrow> _"}$t2$t1;
+
+    fun mk_star' NONE NONE = NONE
+    | mk_star' (SOME t1) NONE  = SOME t1
+    | mk_star' NONE (SOME t2) = SOME t2
+    | mk_star' (SOME t1) (SOME t2) = SOME (mk_star t1 t2);
+
+    fun ptrs_key (_$k$_) = k;
+
+    fun remove_term pt t = case
+      dfs_replace_atomic @{const_name "Groups.times_class.times"} pt 
+        @{term emp} t 
+    of
+      SOME t' => t';  
+
+    fun normalize t = let
+
+      fun ep_tr (has_true,ps,ts,ptrs) t = case t of 
+        Const (@{const_name "pure_assn"},_)$_ 
+        => ((has_true,t::ps,ts,ptrs),NONE)
+      | Const (@{const_name "sngr_assn"},_)$_$_ 
+        => ((has_true,ps,ts,t::ptrs),SOME t)
+      | Const (@{const_name "snga_assn"},_)$_$_
+        => ((has_true,ps,ts,t::ptrs),SOME t)
+      | Const (@{const_name "timeCredit_assn"},_)$_
+        => ((has_true,ps,t::ts,ptrs),NONE)
+      | Const (@{const_name "top_assn"},_)
+        => ((true,ps,ts,ptrs),NONE)
+      | (inf_op as Const (@{const_name "and_assn"},_))$t1$t2
+        => ((has_true,ps,ts,ptrs),SOME (inf_op$normalize t1$normalize t2))
+      | _ => ((has_true,ps,ts,ptrs),SOME t);
+
+      fun normalizer t = case dfs_opr @{const_name "Groups.times_class.times"}
+        ep_tr (false,[],[],[]) t 
+      of 
+        ((has_true,ps,ts,ptrs),rt) => 
+            ((has_true,rev ps,rev ts,ptrs),rt);
+
+      fun normalize_core t = let 
+        val ((has_true,pures,tis,ptrs),rt) = normalizer t;
+        val similar =  find_similar ptrs_key ptrs  ;
+        val true_t = if has_true then SOME @{term "top_assn"} 
+          else NONE;
+        val pures' = case pures of 
+            [] => NONE
+          | p::ps => SOME (fold mk_star ps p);
+        val tis' = case tis of 
+            [] => NONE
+          | p::ps => SOME (fold mk_star ps p);
+      in
+        case similar of NONE => the ((mk_star' pures' (mk_star' tis' (mk_star' true_t rt))) )
+        | SOME (t1,t2) => let
+            val t_stripped = remove_term t1 (remove_term t2 t);
+          in mk_star t_stripped (mk_star t1 t2) 
+          end
+      end;
+
+      fun skip_ex ((exq as Const (@{const_name "ex_assn"},_))$(Abs (n,ty,t))) =
+        exq$Abs (n,ty,skip_ex t)
+      | skip_ex t = normalize_core t;
+
+      val (bs,t') = strip_abs t;
+      val ty = fastype_of1 (map #2 bs,t');
+    in
+      if ty = @{typ assn} then
+        Logic.rlist_abs (bs,skip_ex t')  
+      else t
+    end;
+
+    (*val _ = tracing (tr_term redex);*)
+    val (f,terms) = strip_comb redex;
+    val nterms = map (fn t => let
+        (*val _ = tracing (tr_term t); *)
+        val t'=normalize t; 
+        (*val _ = tracing (tr_term t');*)
+      in t' end) terms;
+    val new_form = list_comb (f,nterms);
+
+    val res_ss = (put_simpset HOL_basic_ss ctxt addsimps @{thms star_aci});
+    val result = Option.map (export o mk_meta_eq) (Arith_Data.prove_conv_nohyps
+      [simp_tac res_ss 1] ctxt' (redex,new_form)
+    );
+
+  in 
+    result
+  end handle exc =>
+    if Exn.is_interrupt exc then Exn.reraise exc
+    else
+      (tracing ("assn_simproc failed with exception\n:" ^ Runtime.exn_message exc);
+        NONE) (* Fail silently *);
+
+
+  val assn_simproc =
+    Simplifier.make_simproc @{context} "assn_simproc"
+     {lhss =
+      [@{term "h \<Turnstile> P"},
+       @{term "P \<Longrightarrow>\<^sub>A Q"},
+       @{term "P \<Longrightarrow>\<^sub>t Q"} ,
+       @{term "hoare_triple P c Q"} (*,
+       @{term "(P::assn) = Q"} *)],
+      proc = K assn_simproc_fun};
+
+
+  (***********************************)
+  (*     Default Simplifications     *)
+  (***********************************)
+
+  (* Default simplification. MUST contain assertion normalization!
+    Tactic must not fail! *)
+  fun dflt_tac ctxt = asm_full_simp_tac
+    (put_simpset HOL_ss ctxt
+      addsimprocs [assn_simproc] 
+      addsimps @{thms norm_assertion_simps}
+      addsimps (Named_Theorems.get ctxt @{named_theorems sep_dflt_simps})
+      |> fold Splitter.del_split @{thms if_split}
+    );
+
+
+  (***********************************)
+  (*         Frame Matcher           *)
+  (***********************************)
+
+  (* Do frame matching
+    imp_solve_tac - tactic used to discharge first assumption of match-rule
+      cf. lemma FI_match.
+  *)
+  fun match_frame_tac imp_solve_tac ctxt = let
+    (* Normalize star-lists *)
+    val norm_tac = simp_tac (
+      put_simpset HOL_basic_ss ctxt addsimps @{thms SLN_normalize});
+
+    (* Strip star-lists *)
+    val strip_tac = 
+      simp_tac (put_simpset HOL_basic_ss ctxt addsimps @{thms SLN_strip}) THEN'
+      simp_tac (put_simpset HOL_basic_ss ctxt addsimps @{thms SLN_def});
+
+    (* Do a match step *)
+    val match_tac = resolve_tac ctxt @{thms FI_match} (* Separate p,q*)
+      THEN' SOLVED' imp_solve_tac (* Solve implication *)
+      THEN' norm_tac;
+
+    (* Do a no-match step *)
+    val nomatch_tac = resolve_tac ctxt @{thms FI_p_nomatch} ORELSE' 
+      (resolve_tac ctxt @{thms FI_q_nomatch} THEN' norm_tac);
+  in
+    resolve_tac ctxt @{thms FI_init} THEN' norm_tac 
+    THEN' REPEAT_DETERM' (FIRST' [
+      CHANGED o dflt_tac ctxt,
+      (match_tac ORELSE' nomatch_tac)])
+    THEN' resolve_tac ctxt @{thms FI_finalize} THEN' strip_tac
+  end;
+
+
+
+  (***********************************)
+  (*         Frame Inference         *)
+  (***********************************)
+
+  fun frame_inference_tac ctxt =
+    resolve_tac ctxt @{thms frame_inference_init} 
+    THEN' match_frame_tac (resolve_tac ctxt @{thms ent_refl}) ctxt
+    THEN' resolve_tac ctxt @{thms frame_inference_finalize};
+
+ 
+
+  (***********************************)
+  (* Nat splitter  powerd by auto2   *)
+  (***********************************)
+
+  fun mytac ctxt a b = let 
+        val _ = tracing (Syntax.string_of_term ctxt a)
+      val _ = tracing (Syntax.string_of_term ctxt b) 
+      val ths = map snd (SepTimeSteps.split_nat ctxt ([], (a, b))); 
+   in
+         (if length ths > 0 then  (EqSubst.eqsubst_tac ctxt [1] ths 
+              THEN' FIRST' [ resolve_tac ctxt @{thms refl}, 
+                             SOLVED' (simp_tac (put_simpset HOL_ss ctxt  addsimps @{thms mult.commute})) ] ) 1  else no_tac) end 
+
+  fun split_nat_tac ctxt =
+     Subgoal.FOCUS_PARAMS (fn {context = ctxt, ...} => ALLGOALS (
+        SUBGOAL (fn (t, _) => case Logic.strip_imp_concl t of
+          @{mpat "Trueprop (?a = ?b + _)"} => 
+            mytac ctxt a b 
+         |  _ => no_tac
+        ))
+      ) ctxt  
+ 
+  (* assumes a goal of form "a = b + c",
+      normalizes a and b using NatRing.norm_full *)
+  fun normalize_time_goal ctxt = 
+     (CONVERSION (Conv.params_conv ~1 (fn _ =>
+              (Conv.concl_conv ~1 
+               (Conv.arg_conv (Conv.every_conv
+              [Conv.arg1_conv(NatRing.norm_full),
+             Conv.arg_conv(Conv.arg1_conv(NatRing.norm_full)),
+             Conv.all_conv])))) ctxt)
+    ) 
+
+
+  (***********************************)
+  (*         Time Frame Inference   *)
+  (***********************************)
+
+  fun print_tac' ctxt i st =
+    let val _ = tracing ("..>");
+        val _ = tracing (Thm.string_of_thm ctxt st)
+    in all_tac st end
+
+  fun time_frame_inference_tac ctxt =
+    TRY o resolve_tac ctxt @{thms timeframe_inference_init_normalize}
+    THEN' 
+    resolve_tac ctxt @{thms timeframe_inference_init} 
+    (* normal frame inference *)
+    THEN' match_frame_tac (resolve_tac ctxt @{thms ent_refl}) ctxt
+
+    THEN' (resolve_tac ctxt @{thms frame_inference_finalize})
+      (* possible non determinism here, countered by the
+        application of safe at the end *)
+    (*THEN' (fn k => print_tac ctxt "aaa")*)
+    THEN'  TRY o (EqSubst.eqsubst_tac ctxt [0] @{thms One_nat_def[symmetric]} ) 
+    THEN'  TRY o (REPEAT_DETERM' (EqSubst.eqsubst_tac ctxt [0] @{thms Suc_eq_plus1} )) 
+
+    THEN' (resolve_tac ctxt @{thms TI_QUERYD}) 
+
+    THEN' normalize_time_goal ctxt  
+
+    THEN' split_nat_tac ctxt
+   
+    THEN' FIRST' [resolve_tac ctxt @{thms refl} ,
+        TRY o (safe_steps_tac ctxt) THEN' resolve_tac ctxt @{thms refl}  ]
+
+    ;
+
+
+  (***********************************)
+  (*       Entailment Solver         *)
+  (***********************************)
+
+  (* Extract existential quantifiers from entailment goal *)
+  fun extract_ex_tac ctxt i st = let
+    fun count_ex (Const (@{const_name SepAuto_Time.entails},_)$_$c) = 
+      count_ex c RS @{thm HOL.mp}
+    | count_ex (Const (@{const_name SepAuto_Time.ex_assn},_)$Abs (_,_,t))
+      = count_ex t RS @{thm enorm_exI'}
+    | count_ex _ = @{thm imp_refl};
+
+    val concl = Logic.concl_of_goal (Thm.prop_of st) i |> HOLogic.dest_Trueprop;
+    val thm = count_ex concl;
+    (* val _ = tracing (Thm.string_of_thm ctxt thm); *)
+  in
+    (TRY o REPEAT_ALL_NEW (match_tac ctxt @{thms ent_ex_preI}) THEN'
+     resolve_tac ctxt [thm]) i st
+  end;
+ 
+
+  fun atom_solve_tac ctxt = 
+        FIRST' [ resolve_tac ctxt @{thms ent_refl},
+                 SOLVED' ( resolve_tac ctxt @{thms dollarD} THEN'
+                             (SELECT_GOAL (auto_tac ctxt))  )
+               ]  
+
+  (* Solve Entailment *)
+  fun solve_entails_tac ctxt = let
+    val preprocess_entails_tac = 
+      dflt_tac ctxt 
+      THEN' extract_ex_tac ctxt
+      THEN' simp_tac 
+        (put_simpset HOL_ss ctxt addsimps @{thms solve_ent_preprocess_simps});
+
+    val match_entails_tac =
+      FIRST' [
+
+      resolve_tac ctxt @{thms entails_solve_init_time} 
+      THEN' match_frame_tac (atom_solve_tac ctxt)  ctxt
+      THEN' resolve_tac ctxt @{thms entails_solve_finalize} 
+      THEN'  TRY o (EqSubst.eqsubst_tac ctxt [0] @{thms One_nat_def[symmetric]} ) 
+      THEN'  TRY o (REPEAT_DETERM' (EqSubst.eqsubst_tac ctxt [0] @{thms Suc_eq_plus1} )) 
+
+      THEN' (resolve_tac ctxt @{thms TI_QUERYD})
+      THEN' normalize_time_goal ctxt  
+      THEN' SOLVED' (split_nat_tac ctxt),
+    
+      resolve_tac ctxt @{thms entails_solve_init} 
+      THEN' match_frame_tac (atom_solve_tac ctxt)  ctxt
+      THEN' resolve_tac ctxt @{thms entails_solve_finalize}
+       ];
+  in
+    preprocess_entails_tac
+    THEN' (TRY o
+      REPEAT_ALL_NEW (match_tac ctxt (rev (Named_Theorems.get ctxt @{named_theorems sep_eintros}))))
+    THEN_ALL_NEW (  dflt_tac ctxt THEN'                                             
+      TRY o (match_tac ctxt @{thms ent_triv} 
+        ORELSE' resolve_tac ctxt @{thms ent_refl}
+        ORELSE' match_entails_tac))
+  end;
+
+
+  (***********************************)
+  (* Verification Condition Generator*)
+  (***********************************)
+
+  fun heap_rule_tac ctxt h_thms =  
+    resolve_tac ctxt h_thms ORELSE' (
+    resolve_tac ctxt @{thms fi_rule} THEN' (resolve_tac ctxt h_thms THEN_IGNORE_NEWGOALS
+    ( dflt_tac ctxt (*THEN' (fn k => print_tac ctxt "AAAH")*) THEN'  time_frame_inference_tac ctxt) ))                                           
+
+  (* Apply consequence rule if postcondition is not a schematic var *)
+  fun app_post_cons_tac ctxt i st = 
+    case Logic.concl_of_goal (Thm.prop_of st) i |> HOLogic.dest_Trueprop of
+      Const (@{const_name hoare_triple},_)$_$_$qt =>
+        if is_Var (head_of qt) then no_tac st
+        else resolve_tac ctxt @{thms cons_post_rule} i st
+    | _ => no_tac st;
+
+  fun vcg_step_tac ctxt = let
+    val h_thms = rev (Named_Theorems.get ctxt @{named_theorems sep_heap_rules});
+    val d_thms = rev (Named_Theorems.get ctxt @{named_theorems sep_decon_rules});
+    val heap_rule_tac = heap_rule_tac ctxt h_thms
+
+  in
+    CSUBGOAL (snd #> (FIRST' [
+      CHANGED o dflt_tac ctxt,
+      REPEAT_ALL_NEW (resolve_tac ctxt @{thms normalize_rules}),
+      CHANGED o (FIRST' [resolve_tac ctxt d_thms, heap_rule_tac]
+        ORELSE' (app_post_cons_tac ctxt THEN' 
+          FIRST' [resolve_tac ctxt d_thms, heap_rule_tac])) 
+    ]))
+  end; 
+  fun vcg_tac ctxt = REPEAT_DETERM' (  vcg_step_tac ctxt)
+                                          
+ 
+
+  (***********************************)
+  (*        Automatic Solver         *)
+  (***********************************)
+
+  fun sep_autosolve_tac do_pre do_post ctxt = let
+    val pre_tacs = [
+      CHANGED o (clarsimp_tac ctxt),
+      CHANGED o (REPEAT_ALL_NEW (match_tac ctxt @{thms ballI allI impI conjI}))
+    ];                                
+    val main_tacs = [
+      match_tac ctxt @{thms is_hoare_triple} THEN' CHANGED o vcg_tac ctxt,
+      match_tac ctxt @{thms is_entails} THEN' CHANGED o solve_entails_tac ctxt
+    ];                                                       
+    val post_tacs = [   SELECT_GOAL (auto_tac ctxt)];
+    val tacs = (if do_pre then pre_tacs else [])
+      @ main_tacs 
+      @ (if do_post then post_tacs else []);
+  in
+    REPEAT_DETERM' (CHANGED o FIRST' tacs)
+  end;
+
+  fun sep_step_autosolve_tac do_pre do_post ctxt = let
+    val pre_tacs = [
+      CHANGED o (clarsimp_tac ctxt),
+      CHANGED o (REPEAT_ALL_NEW (match_tac ctxt @{thms ballI allI impI conjI}))
+    ];                                
+    val main_tacs = [
+      match_tac ctxt @{thms is_hoare_triple} THEN' CHANGED o vcg_step_tac ctxt,
+      match_tac ctxt @{thms is_entails} THEN' CHANGED o solve_entails_tac ctxt
+    ];                                                       
+    val post_tacs = [   SELECT_GOAL (auto_tac ctxt)];
+    val tacs = (if do_pre then pre_tacs else [])
+      @ main_tacs 
+      @ (if do_post then post_tacs else []);
+  in
+      (CHANGED o FIRST' tacs)
+  end;
+
+ 
+
+
+end; \<open>struct\<close>
+
+
+\<close>  
+
+method_setup vcg = \<open>
+  Scan.lift (Args.mode "ss") --
+  Method.sections Seplogic_Auto.vcg_modifiers >>
+  (fn (ss,_) => fn ctxt => SIMPLE_METHOD' (
+  CHANGED o (
+    if ss then Seplogic_Auto.vcg_step_tac ctxt 
+    else Seplogic_Auto.vcg_tac ctxt
+  )
+))\<close> "Seplogic: Verification Condition Generator"
+
+method_setup sep_auto = 
+  \<open>Scan.lift (Args.mode "nopre" -- Args.mode "nopost" -- Args.mode "plain") 
+      --| Method.sections Seplogic_Auto.sep_auto_modifiers >>
+  (fn ((nopre,nopost),plain) => fn ctxt => SIMPLE_METHOD' (
+    CHANGED o Seplogic_Auto.sep_autosolve_tac 
+      ((not nopre) andalso (not plain)) 
+      ((not nopost) andalso (not plain)) ctxt
+  ))\<close> "Seplogic: Automatic solver"
+
+method_setup sep_auto_step = 
+  \<open>Scan.lift (Args.mode "nopre" -- Args.mode "nopost" -- Args.mode "plain") 
+      --| Method.sections Seplogic_Auto.sep_auto_modifiers >>
+  (fn ((nopre,nopost),plain) => fn ctxt => SIMPLE_METHOD' (
+    CHANGED o Seplogic_Auto.sep_step_autosolve_tac 
+      ((not nopre) andalso (not plain)) 
+      ((not nopost) andalso (not plain)) ctxt
+  ))\<close> "Seplogic: Automatic solver"
+
+method_setup solve_entails = \<open>
+  Method.sections Seplogic_Auto.solve_entails_modifiers >>
+  (fn _ => fn ctxt => SIMPLE_METHOD' (
+  CHANGED o Seplogic_Auto.solve_entails_tac ctxt
+))\<close> "Seplogic: Entailment Solver"
+
+method_setup time_frame_inference = \<open>
+  Method.sections Seplogic_Auto.solve_entails_modifiers >>
+  (fn _ => fn ctxt => SIMPLE_METHOD' (
+  CHANGED o Seplogic_Auto.time_frame_inference_tac ctxt
+))\<close> "Seplogic: Frame Inference with Time Inference"
+ 
+method_setup frame_inference = \<open> 
+  Method.sections Seplogic_Auto.solve_entails_modifiers >>
+  (fn _ => fn ctxt => SIMPLE_METHOD' (
+  CHANGED o Seplogic_Auto.frame_inference_tac ctxt
+)) \<close> "Seplogic: Frame Inference without Time Inference"
+
+simproc_setup assn_simproc 
+  ( "h \<Turnstile> P" | "P\<Longrightarrow>\<^sub>AQ" | "P\<Longrightarrow>\<^sub>tQ" | "(P::assn) = Q" ) 
+  = \<open>K Seplogic_Auto.assn_simproc_fun\<close>
+
+
+subsection \<open>Examples and Regression Tests\<close>
+
+lemma " P * $ 0 \<Longrightarrow>\<^sub>A P * true "
+  by (solve_entails)
+
+lemma " P * $ 1 \<Longrightarrow>\<^sub>A P * true * $ 1"
+  by (solve_entails)
+
+lemma "QA \<Longrightarrow> (P \<Longrightarrow>\<^sub>A \<exists>\<^sub>Ax. Q x)"
+      apply(tactic \<open>IF_EXGOAL (Seplogic_Auto.extract_ex_tac @{context}) 1\<close>)
+  oops
+
+  thm new_rule
+schematic_goal "\<And>x. P \<Longrightarrow> Q \<Longrightarrow>   <x \<mapsto>\<^sub>a [0..<n] * $ (n * 15 + 11)> Array_Time.new n 0 <?Q18 x>"
+  by (sep_auto heap: new_rule)
+
+
+lemma "\<And>x. x \<mapsto>\<^sub>a replicate (N * M) 0 * timeCredit_assn ((M * N * 9))  * timeCredit_assn (2) \<Longrightarrow>\<^sub>A x \<mapsto>\<^sub>a replicate (N * M) 0 * timeCredit_assn (Suc (Suc (9 * (N * M))))"
+  by (solve_entails)
+
+
+schematic_goal "\<And>end start' start_next x' k k_next start'a start_nexta x'a enda start'b start_nextb x'b ka k_nexta start'c start_nextc x'c.
+       start_nextc = Some p' \<and>
+       k_nexta = enda \<and> k_nexta = Some start'c \<and> p' = start'b \<and> start_nexta = Some q' \<and> k_next = end \<and> k_next = Some start'a \<and> q' = start' \<Longrightarrow>
+       <start'b \<mapsto>\<^sub>r Cell x'b start_nextb enda * R a x'b *
+        (dll_seg R cs' start_nextb (Some start'b) ka enda *  
+        (start' \<mapsto>\<^sub>r Cell x' start_next end * R u x' * (dll_seg R vs' start_next (Some start') k end * (start'a \<mapsto>\<^sub>r Cell x'a (Some start') k * R w x'a)))) *
+        $ 1>
+       !start'b <?Q20 end start' start_next x' k end start'a (Some start') x'a enda start'b start_nextb x'b ka enda start'c (Some start'b) x'c>"
+  apply (vcg (ss) heap: lookup_rule) oops
+
+declare entt_refl' [simp]
+
+lemma "\<And>x. M = 0 \<Longrightarrow> (\<And>j i. c (i, j) = 0) \<Longrightarrow> x \<mapsto>\<^sub>a [] \<Longrightarrow>\<^sub>A \<exists>\<^sub>Al. x \<mapsto>\<^sub>a l * true * \<up> (l = []) "
+  apply(sep_auto)  
+  done
+
+
+
+schematic_goal "timeCredit_assn (B* A * 10 + 3) \<Longrightarrow>\<^sub>A ?F1 * timeCredit_assn (B* A + 1)"
+  by time_frame_inference  
+ 
+schematic_goal "ya \<mapsto>\<^sub>r Cell x' (Some end) (Some end) * (R x x' * end \<mapsto>\<^sub>r Cell y' (Some ya) (Some ya) * R y y') * $ 9 \<Longrightarrow>\<^sub>A
+        ?F62 end x' y' (Cell x' (Some end) (Some end)) ya * $ 1"
+  by time_frame_inference  
+
+schematic_goal "\<And>end x' y' xa ya.
+       p = Some ya \<Longrightarrow>
+       xa = Cell x' (Some end) (Some end) \<Longrightarrow>
+       Some ya \<noteq> Some end \<Longrightarrow>
+       ya \<mapsto>\<^sub>r Cell x' (Some end) (Some end) * (R x x' * end \<mapsto>\<^sub>r Cell y' (Some ya) (Some ya) * R y y') * $ 9 \<Longrightarrow>\<^sub>A
+       ?F62 end x' y' (Cell x' (Some end) (Some end)) ya * $ 1"
+  apply time_frame_inference done
+
+
+(* timeframeinf can solve problems of that form: A * $T \<Longrightarrow>\<^sub>A B * ?F * $T' *)
+schematic_goal "\<up> (i < length xs) * a \<mapsto>\<^sub>a xs *  $2  \<Longrightarrow>\<^sub>A a \<mapsto>\<^sub>a xs * ?F * $1"  
+  by time_frame_inference
+
+schematic_goal "A * C * $2  \<Longrightarrow>\<^sub>A A * ?F * $1"  
+  by time_frame_inference
+
+schematic_goal "a \<mapsto>\<^sub>a xs * $ 1 \<Longrightarrow>\<^sub>A a \<mapsto>\<^sub>a xs * ?F24 (xs ! i)   * $ 1"  
+  by time_frame_inference 
+thm mult_1
+
+schematic_goal "a \<mapsto>\<^sub>a xs * $ (2 + 3 * ff + (5 * (3*ff+2)))
+           \<Longrightarrow>\<^sub>A a \<mapsto>\<^sub>a xs * ?F24   * $ (1 + ff * 2 + 4 * ff)"  
+  by time_frame_inference 
+
+
+context begin
+  definition "fffa = (10::nat)"
+ 
+lemma "F * $(xx*(3+7+yy)) \<Longrightarrow>\<^sub>A F * $(xx*2+yy*xx) * true"
+  by (solve_entails) 
+  
+
+  schematic_goal "(3::nat) + 3 * fffa + 6 * 7 = 1 + ?F"
+    apply(tactic \<open>Seplogic_Auto.split_nat_tac @{context} 1\<close>)
+    done
+  
+  schematic_goal "(2::nat) + 3 * fffa  = 1 + ?F"
+    apply(tactic \<open>Seplogic_Auto.split_nat_tac @{context} 1\<close>)
+    done
+
+  schematic_goal "(2::nat) + fffa * 32 = 1 + fffa * 1 + ?F"
+    apply(tactic \<open>Seplogic_Auto.normalize_time_goal @{context} 1\<close>)
+    apply(tactic \<open>Seplogic_Auto.split_nat_tac @{context} 1\<close>)
+    done
+
+  schematic_goal "(2::nat) + 3 * fffa  = 1 + 2 * fffa + ?F"
+    apply(tactic \<open>Seplogic_Auto.normalize_time_goal @{context} 1\<close>)
+    apply(tactic \<open>Seplogic_Auto.split_nat_tac @{context} 1\<close>)
+    done
+end 
+
+
+
+lemma "A \<Longrightarrow>\<^sub>A A"
+  by solve_entails
+
+
+lemma "A * B \<Longrightarrow>\<^sub>A A * true"
+  by solve_entails  
+
+lemma "A * B * C \<Longrightarrow>\<^sub>A B * A * true"
+  by solve_entails
+
+
+
+
+
+lemma "$a * $b = $(a+b)"  
+  by (simp add: time_credit_add)
+
+lemma "$1* \<up>g * G * $2 * $3 *true * F * true * \<up>ff * $4 * $5 = G * F * true * $ 10 * (\<up> g *  $5 * \<up> ff)"
+  by (simp add : time_credit_add[symmetric] )  
+
+lemma "G * \<up>ff * true *  F   = H"  apply (simp )   oops
+
+lemma "h \<Turnstile> F \<and>\<^sub>A \<up> (a' = None) * F' \<Longrightarrow> G" apply simp oops
+
+lemma "h \<Turnstile> \<up>t * (F \<and>\<^sub>A \<up> (a' = None) * F') * X \<Longrightarrow> G" apply (simp del:  ) oops
+
+
+lemma p_c[simp]: "\<up> P * \<up> Q = \<up> (P \<and> Q)" using pure_conj by simp
+
+lemma "\<up>a * B * \<up>c \<Longrightarrow>\<^sub>A G" apply (simp add:  del: pure_conj) oops
+
+
+lemma "\<exists>\<^sub>Ab. \<up> ((b, a) \<in> R) *C *\<up>a \<Longrightarrow>\<^sub>A emp" apply simp oops
+
+
+lemma "P * $4 \<Longrightarrow>\<^sub>A P * true * $3"
+    "P * $3 \<Longrightarrow>\<^sub>A P * true"
+    "P * Q *  $(f x * 4 + 3) \<Longrightarrow>\<^sub>A Q * P * true * $(f x * 4)"
+    "P * Q *  $(g y * 6 + f x * 4 + 3) \<Longrightarrow>\<^sub>A Q * P * true * $(g y * 2 + f x * 4)"
+  by solve_entails+
+
+
+lemma "\<And>x. x \<mapsto>\<^sub>a replicate (N * M) 0 * $ ((M * N * 9))  * $ (2)
+       \<Longrightarrow>\<^sub>A x \<mapsto>\<^sub>a replicate (N * M) 0 * $ (Suc (Suc (9 * (N * M))))"
+  by (sep_auto) 
+
+
+lemma "\<And>x. x \<mapsto>\<^sub>a replicate (N * M) 0 * $ ((M * N * 9))  * $ (2)
+         \<Longrightarrow>\<^sub>A x \<mapsto>\<^sub>a replicate (N * M) 0 * timeCredit_assn (Suc (Suc (9 * (N * M))))"
+  apply(vcg (ss))
+  by (sep_auto)
+
+
+subsection \<open>setup sep_auto rules\<close>
+
+thm sep_eintros
+
+lemma ureturn_rule: "<P> ureturn x <\<lambda>r. P * \<up>(r = x)>" 
+  apply(rule post_rule)
+  apply(rule pre_rule[rotated])
+    apply(rule frame_rule[OF return_rule, where R=P] )
+  by auto
+
+(* sep auto expects pure assertions to be pulled out in the pre condition TODO: is this correct? *)
+lemma nth_rule'[sep_heap_rules]:
+  "(i < length xs) \<Longrightarrow> <a \<mapsto>\<^sub>a xs * $ 1 > Array_Time.nth a i <\<lambda>r. a \<mapsto>\<^sub>a xs * \<up> (r = xs ! i)>"
+  apply(rule pre_rule[OF _ nth_rule]) by sep_auto
+
+lemma upd_rule': "i < length xs \<Longrightarrow> <a \<mapsto>\<^sub>a xs * timeCredit_assn 1 > Array_Time.upd i x a <\<lambda>r. a \<mapsto>\<^sub>a xs[i := x] * \<up> (r = a)>"
+  apply(rule pre_rule[OF _ upd_rule])  
+  by solve_entails
+
+lemma assert_rule_alt: 
+  "(Q \<Longrightarrow>\<^sub>A true * \<up>(P x)) \<Longrightarrow>
+     <Q * $1> assert P x <\<lambda> _. Q * \<up>(P x)>"
+  unfolding assert_def
+  apply (sep_auto heap: SepAuto_Time.return_rule decon: assert_rule)
+  unfolding hoare_triple_def
+  using mod_starD by blast
+
+
+
+lemma option_rule:
+  assumes "p = None \<Longrightarrow> <P> f <Q>"
+  assumes "\<And> x. p = Some x \<Longrightarrow> <P> g x <Q>"
+  shows "<P> case p of None \<Rightarrow> f | Some x \<Rightarrow> g x <Q>"
+  using assms by (sep_auto split: option.splits)
+
+lemma prod_rule:
+  assumes "\<And> x y. z = (x, y) \<Longrightarrow> <P> g x y <Q>"
+  shows "<P> case z of (x, y) \<Rightarrow> g x y <Q>"
+  using assms by (sep_auto split: prod.splits)
+
+lemma prod_pre_split: 
+  assumes "\<And> x y. <P x y * \<up> (p = (x, y))> f <Q>"
+  shows "<case p of (x, y) \<Rightarrow> P x y> f <Q>"
+proof (cases p)
+  case [simp]: (Pair x y)
+  have "P x y * \<up> (p = (x, y)) = (case p of (x, y) \<Rightarrow> P x y)" by simp
+  then show ?thesis using assms[of x y] by simp
+qed
+
+lemmas prod_split_rule = prod_rule
+
+
+lemma If_rule:
+  "(b \<Longrightarrow> <P> f <Q>) \<Longrightarrow> (\<not> b \<Longrightarrow> <P> g <Q>) \<Longrightarrow> <P> if b then f else g <Q>"
+  by auto 
+
+lemma Let_rule: "(\<And>x. x = t \<Longrightarrow> <P> f x <Q>) \<Longrightarrow> <P> Let t f <Q>" 
+  by simp
+
+
+lemma prod_case_simp[sep_dflt_simps]:
+  "(case (a, b) of (c, d) \<Rightarrow> f c d) = f a b" by simp
+
+
+lemmas [sep_decon_rules] = 
+          assert_rule bind_rule ureturn_rule Let_rule If_rule
+          option_rule prod_rule prod_pre_split
+                 
+lemmas [sep_heap_rules] =
+          length_rule SepAuto_Time.return_rule
+          new_rule make_rule
+          ref_rule lookup_rule upd_rule'
+          update_rule 
+          assert_rule_alt
+
+
+thm upd_rule'
+
+lemmas [sep_eintros] = impI conjI exI
+   
+subsection \<open>examples for sep_auto\<close>
+      
+schematic_goal "<$ 1> Array_Time.new 0 0 <?Q8>"
+  by sep_auto
+
+
+subsection \<open>BUGS and Ideas for enhancements\<close>
+
+text \<open>time_frame_inference has the invariant, that the last
+    component in the symbolic heap is a time credit.
+    once such a time credit is not available the method breaks,
+    this occurs for example, when an operation has no advertised cost
+    while using sep_auto.
+    e.g. in fibonacci/Doubly_Linked_List_With_Time : dll_fold_rule_weak\<close>
+schematic_goal " xs\<^sub>2 = [] \<Longrightarrow>
+          A * (B * F) * $ (Suc (Suc 0)) \<Longrightarrow>\<^sub>A
+          B * F * ?R * $0" 
+  apply time_frame_inference oops
+
+schematic_goal " xs\<^sub>2 = [] \<Longrightarrow>
+          A * (B * F) * $ (Suc (Suc 0)) \<Longrightarrow>\<^sub>A
+          B * F * ?R "   oops
+
+
+
+end
