SepLogicTime/Sep_Time_Main.thy
@@ -1,0 +1,8 @@
+section \<open>Separation Logic for Imperative HOL with Time Entrypoint\<close>
+theory Sep_Time_Main
+imports "Sep_Time_Automation"
+begin
+text \<open>Import this theory to make available separation logic for 
+  Imperative-HOL with time.\<close>
+end
+
