ROOT
@@ -1,6 +1,7 @@
 chapter Imperative_HOL_Time
 
-session SepLogicTime_Base = HOL +
+
+session SepLogicTime_Prereq in "SepLogicTime_Prereq" = HOL +
   sessions
     Auto2_Imperative_HOL
     Berlekamp_Zassenhaus
@@ -14,37 +15,66 @@ session SepLogicTime_Base = HOL +
     "Amortized_Complexity.Skew_Heap_Analysis"
     "Median_Of_Medians_Selection.Median_Of_Medians_Selection"
 
-session SepLogicTime_Fun = SepLogicTime_Base +
-  description \<open>
-    Functional algorithms
-\<close>
-  sessions
-    Auto2_HOL
-  theories
-    "Functional/BinarySearch"
-    "Functional/MergeSort"
-    "Functional/Select"
-    "Functional/Karatsuba"
-    "Functional/Knapsack"
-
-session SepLogicTime_Impl = SepLogicTime_Fun +
+(* Session with all the Examples in Imperative HOL Time *)
+session Imperative_HOL_Time = SepLogicTime_Prereq +
   description \<open>
     Separation logic with time.
 \<close>
   sessions
-    Auto2_HOL
+    "HOL-Imperative_HOL"
+    "HOL-Library"
+  directories
+    "Examples"
+    "Asymptotics"
+    "SepLogicTime"
+    "Functional"
   theories
-    "SepLogicTime/Sep_Time_Examples"
-
-session Imperative_HOL_Time = SepLogicTime_Base +
-  sessions
-    Auto2_HOL
-  theories
-    "SepLogicTime/RBTree_Impl"
-    "SepLogicTime/LinkedList"
-    "SepLogicTime/DynamicArray2"
-    "Asymptotics/Asymptotics_2D"
-    "SepLogicTime/MergeSort_Impl"
+    "Sep_Time_Examples"
     "Sep_Time_Main"
-    
+
+(* smaller sessions *)
+session Imperative_HOL_Time_Base in "Imperative_HOL_Time_Base" = HOL +
+  sessions
+    "Imperative_HOL_Time"
+  theories
+    "Imperative_HOL_Time.Imperative_HOL_Time"
+
+session SepLogicTime_Base in "SepLogicTime_Base" =  Imperative_HOL_Time_Base +
+  sessions
+    Imperative_HOL_Time
+  theories
+    "Imperative_HOL_Time.Sep_Time_Main"
+
+session SepLogicTime_Asymptotics in "SepLogicTime_Asymptotics" = Akra_Bazzi +
+  sessions
+    Imperative_HOL_Time
+  theories
+    "Imperative_HOL_Time.Asymptotics_Test"
+
+session SepLogicTime_Fun in "SepLogicTime_Fun" = SepLogicTime_Prereq +
+  description \<open>
+    Functional algorithms
+\<close>
+  sessions
+    Imperative_HOL_Time
+  theories
+    "Imperative_HOL_Time.BinarySearch"
+    "Imperative_HOL_Time.MergeSort"
+    "Imperative_HOL_Time.Select"
+    "Imperative_HOL_Time.Karatsuba"
+    "Imperative_HOL_Time.Knapsack"
+
+(* Session with a limited number of Data Structures and simple Algorithms.
+    Does not contain all the examples
+    Serves as entry point for Separation Logic for Imperative-HOL-Time. *)
+session Imperative_HOL_Time_Entry in "SepLogicTime_Entry" = SepLogicTime_Fun +
+  sessions
+    Imperative_HOL_Time
+  theories
+    "Imperative_HOL_Time.RBTree_Impl"
+    "Imperative_HOL_Time.LinkedList"
+    "Imperative_HOL_Time.DynamicArray2"
+    "Imperative_HOL_Time.Asymptotics_2D"
+    "Imperative_HOL_Time.MergeSort_Impl"
+    "Imperative_HOL_Time.Sep_Time_Main"
                       
